WIP trying to fix byte reg

examples/byte_register.thy
@@ -36,12 +36,8 @@ definition ST
 
 (* DBL doubles the number, if it is low enough to double without overflow *)
 definition DBL
-  where "DBL = (reg\<^sup>< \<ge> 0 \<and> reg\<^sup>< \<le> 127 \<and> err\<^sup>< = 0)\<^sub>e \<turnstile>\<^sub>r (reg\<^sup>> = reg\<^sup>< * 2 \<and> err\<^sup>> = 0)\<^sub>e"
-
-value "DBL (\<lparr> ok\<^sub>v = True, \<dots> = \<lparr> reg\<^sub>v = -1, err\<^sub>v = 0 \<rparr> \<rparr>, \<lparr> ok\<^sub>v = False, \<dots> = \<lparr> reg\<^sub>v = 0, err\<^sub>v = 0 \<rparr> \<rparr>)"
-
-value "ucast (drop_bit 4 (240::8 word)) :: 4 word"
-value "ucast (take_bit 4 (15::8 word)) :: 4 word"
+(*  where "DBL = (reg\<^sup>< \<ge> 0 \<and> reg\<^sup>< \<le> 127 \<and> err\<^sup>< = 0)\<^sub>e \<turnstile>\<^sub>r (reg\<^sup>> = reg\<^sup>< * 2 \<and> err\<^sup>> = 0)\<^sub>e"*)
+  where "DBL = (reg \<ge> 0 \<and> reg \<le> 127 \<and> err = 0) \<turnstile>\<^sub>n (reg\<^sup>> = reg\<^sup>< * 2 \<and> err\<^sup>> = 0)\<^sub>e"
 
 (* A view of the high nibble *)
 definition Hv
@@ -50,6 +46,13 @@ definition Hv
 (* A view of the low nibble *)
 definition Lv
   where "Lv = OK (((vu:reg\<^sub>L = (ucast (take_bit 4 sys:reg))) \<and> (vu:err\<^sub>L = sys:err))\<^sub>e \<up> \<^bold>v\<^sub>D)"
+
+(* These are both healthy *)
+lemma hv_is_vhd: "Hv is VHD"
+  by (pred_auto_banks add: Hv_def)
+
+lemma lv_is_vhd: "Lv is VHD"
+  by (pred_auto_banks add: Lv_def)
 
 (*
 Consider an example where the register stores the value 60
@@ -60,12 +63,6 @@ Here is an observation on the final state, with this value
 *)
 
 definition \<Phi> where "\<Phi> = (reg = 60 \<and> err = 0)\<^sub>e"
-
-lemma hv_is_vhd: "Hv is VHD"
-  by (pred_auto_banks add: Hv_def)
-
-lemma "Lv is VHD"
-  by (pred_auto_banks add: Lv_def)
 
 (*
   Hv and Lv extract the high nibble and low nibble, respectively
@@ -80,34 +77,47 @@ lemma "(((L (Hv \<down> \<^bold>v\<^sub>D) (\<Delta> \<Phi>))) \<down> vu\<^sup>
 lemma "(((L (Lv \<down> \<^bold>v\<^sub>D) (\<Delta> \<Phi>))) \<down> vu\<^sup>2) = \<Delta> (reg\<^sub>L = 12 \<and> err\<^sub>L = 0)\<^sub>e"
   by (pred_auto_banks add: Lv_def \<Phi>_def)
 
-term "(as_design_view(
-     ((reg\<^sub>H\<^sup>< \<ge> 0 \<and> reg\<^sub>H\<^sup>< \<le> 7 \<and> err\<^sub>H\<^sup>< = 0)\<^sub>e)
-     \<turnstile>\<^sub>r
-     ((((reg\<^sub>H\<^sup>> = (reg\<^sub>H\<^sup>< * 2)) \<or> (reg\<^sub>H\<^sup>> = ((reg\<^sub>H\<^sup>< * 2) + 1))) \<and> err\<^sub>H\<^sup>> = 0)\<^sub>e)
-  ))"
+definition Loc_H_DBL where "Loc_H_DBL = (L\<^sub>D (Hv) (DBL))"
+definition Loc_L_DBL where "Loc_L_DBL = (L\<^sub>D (Lv) (DBL))"
 
-value "(255::8 word) = (-1::8 word)"
-(*
-lemma "(L\<^sub>D (Hv) (DBL)) (
-        \<lparr> ok\<^sub>v = True, \<dots> = \<lparr> sys\<^sub>v = \<lparr> reg\<^sub>v = 255, err\<^sub>v = 0 \<rparr>, vu\<^sub>v = \<lparr> reg\<^sub>H\<^sub>v = 0, err\<^sub>H\<^sub>v = 0 \<rparr> \<rparr> \<rparr>
-        ,\<lparr> ok\<^sub>v = False, \<dots> = \<lparr> sys\<^sub>v = \<lparr> reg\<^sub>v = 255, err\<^sub>v = 0 \<rparr>, vu\<^sub>v = \<lparr> reg\<^sub>H\<^sub>v = 0, err\<^sub>H\<^sub>v = 0 \<rparr> \<rparr> \<rparr>
-    )"
-  apply (pred_auto_banks add: Hv_def DBL_def)
-  quickcheck
-  apply transfer
-  apply simp
-  *)
+lemma drop_word_lt_div: "(r :: 8 word) \<le> a \<longrightarrow> (drop_bit k r) \<le> a div 2^k"
+  by (simp add: drop_bit_eq_div word_le_nat_alt unat_div_distrib div_le_mono)
 
-term "(L\<^sub>D (Hv) (DBL))"
+term "pre\<^sub>D(Loc_H_DBL)"
 
-find_theorems "take_bit ?n (drop_bit ?m ?P)"
-
-
-lemma "L\<^sub>p ((vu:reg\<^sub>H = (ucast (drop_bit 4 sys:reg))) \<and> (vu:err\<^sub>H = sys:err))\<^sub>e (reg \<ge> 0 \<and> reg \<le> 127 \<and> err = 0)\<^sub>e  = (reg\<^sub>H \<ge> 0 \<and> reg\<^sub>H \<le> 7 \<and> err\<^sub>H = 0)\<^sub>e"
+lemma "pre\<^sub>D(Loc_H_DBL) = true"
+  apply (subst Loc_H_DBL_def)
+  apply (subst pre_design_def)
+  apply (subst banks_defs Hv_def DBL_def)+
   apply (pred_simp add: banks_defs)
+  apply pred_auto
+
+(*lemma "pre\<^sub>D(Loc_H_DBL) = \<Delta> ((reg\<^sub>H \<ge> 0 \<and> reg\<^sub>H \<le> 7 \<and> err\<^sub>H = 0)\<^sub>e \<up> vu)"*)
+lemma "(pre\<^sub>D(Loc_H_DBL) \<down> vu\<^sup>2) = ((reg\<^sub>H\<^sup>< \<ge> 0 \<and> reg\<^sub>H\<^sup>< \<le> 7 \<and> err\<^sub>H\<^sup>< = 0)\<^sub>e)"
+  apply (subst Loc_H_DBL_def)
+  apply (subst pre_design_def)
+  apply (subst banks_defs Hv_def DBL_def)+
+  apply (pred_simp add: drop_word_lt_div)
+    apply transfer
   apply (simp add: drop_bit_eq_div word_le_nat_alt unat_div_distrib div_le_mono)
+  apply auto
 
 
+  value "take_bit 2 4::(4 word)"
+
+lemma "(take_bit 2 3::(4 word)) = 3"
+  apply unat_arith
+  apply smt
+
+lemma "pre\<^sub>D(Loc_L_DBL) = false"
+  apply (subst Loc_L_DBL_def)
+  apply (subst pre_design_def)
+  apply (subst banks_defs Lv_def DBL_def)+
+  apply pred_auto
+  apply unat_arith
+  apply simp
+  apply smt
+  
 
 (* TODO is this right? *)
 lemma
@@ -127,18 +137,19 @@ lemma
    apply pred_simp
   
   apply (pred_auto_banks add: Hv_def DBL_def)
-                      apply (transfer, auto)
-  quickcheck
+          apply (transfer, auto) defer
+          apply (transfer, auto) defer
+          apply (transfer, auto) defer
+          apply (transfer, auto) defer
+          apply (transfer, auto) defer
+          apply (transfer, auto) defer
+          apply (transfer, auto) defer
+          apply (transfer, auto) defer
+          apply (transfer, auto) defer
+  apply smt
 
-lemma "(L\<^sub>D (Hv) (DBL)) (
-   \<lparr> ok\<^sub>v = True, \<dots> = \<lparr> sys\<^sub>v = \<lparr> reg\<^sub>v = 255, err\<^sub>v = 0 \<rparr>, vu\<^sub>v = \<lparr> reg\<^sub>H\<^sub>v = 0, err\<^sub>H\<^sub>v = 0 \<rparr> \<rparr>  \<rparr>
-  ,\<lparr> ok\<^sub>v = False, \<dots> = \<lparr> sys\<^sub>v = \<lparr> reg\<^sub>v = 255, err\<^sub>v = 0 \<rparr>, vu\<^sub>v = \<lparr> reg\<^sub>H\<^sub>v = 0, err\<^sub>H\<^sub>v = 0 \<rparr> \<rparr>  \<rparr>
-)"
-  apply (pred_auto_banks add: Hv_def DBL_def)
-  apply transfer
-  by (metis not_mod_2_eq_0_eq_1 take_bit_eq_mod take_bit_length_eq word_mod_def word_of_int_eq_iff)
 
-lemma "(reg\<^sub>H \<ge> 0 \<and> reg\<^sub>H \<le> 7 \<and> err\<^sub>H = 0)\<^sub>e \<lparr> reg\<^sub>H\<^sub>v = 0, err\<^sub>H\<^sub>v = 0 \<rparr>"
+
 
 lemma " (as_design_view(
     ((reg\<^sub>H\<^sup>< \<ge> 0 \<and> reg\<^sub>H\<^sup>< \<le> 7 \<and> err\<^sub>H\<^sup>< = 0)\<^sub>e)
@@ -161,14 +172,24 @@ lemma "
   ) \<down> \<^bold>v\<^sub>D\<^sup>2
   "
   apply (pred_auto_banks add: Hv_def DBL_def)
-  quickcheck
 
-lemma "(L\<^sub>D (Lv) (DBL)) = true"
-  apply (pred_auto_banks add: DBL_def Lv_def)
-  apply transfer
   nitpick
-  apply smt
 
+
+
+term pre_design
+
+lemma loc_l_dbl_pre_false: "(pre\<^sub>D(LocLDBL)) = false"
+  apply (subst LocLDBL_def, subst pre_design_def, subst L\<^sub>D_def)
+  apply (pred_auto_banks)
+  apply (pred_auto_banks add: DBL_def Lv_def LocLDBL_def)
+
+lemma "LocLDBL = true"
+proof -
+  have "LocLDBL = false \<turnstile> a"
+    apply (pred_auto_banks add: loc_l_dbl_pre_false)
+  apply (subst LocLDBL_def)
+  apply (subst L\<^sub>D_def)
 
 (* DBL2 doubles the number, if it is low enough to double without overflow, but unlike DBL, it
 explicitly defines the behaviour in the overflow case. If overflow is detected, then the err bit is
